Axioms.v
@@ -3,49 +3,55 @@ Require Import Top0.Definitions.
 Require Import Top0.Heap.
 Require Import Top0.Keys.
 
+(* Use these as constructors inside "Inductive Phi" *)
 Axiom Phi_Seq_Nil_L : forall phi, Phi_Seq Phi_Nil phi = phi.
 Axiom Phi_Seq_Nil_R : forall phi, Phi_Seq phi Phi_Nil = phi.
 Axiom Phi_Par_Nil_R : forall phi, Phi_Par phi Phi_Nil = phi.
 Axiom Phi_Par_Nil_L : forall phi, Phi_Par Phi_Nil phi = phi.
 
-Axiom EvaluationMuAppIncludesEffectEvaluation:
-  forall h'' env rho ef fheap env' rho' f x ec' ee' facts ea aheap v v' aacts h' bacts eff
-         facts1 aacts1 bacts1, 
-    (h'', env, rho, ef) ⇓ (fheap, Cls (env', rho', Mu f x ec' ee'), facts) ->
-    (fheap, env, rho, ea) ⇓ (aheap, v, aacts) ->
-    (aheap, update_rec_E (f, Cls (env', rho', Mu f x ec' ee')) (x, v) env', rho', ec') ⇓ (h', v', bacts)->
-    (h'', env, rho, Eff_App ef ea) ⇓ (h'', eff, Phi_Seq (Phi_Seq facts1 aacts1) bacts1) ->
-    (h'', update_rec_E (f, Cls (env', rho', Mu f x ec' ee')) (x, v) env', rho', ee') ⇓ (h'', eff, bacts1).
+ (* both ec' and ee' and evaluated with the same context, but twice: inside Bs_Mu_App and BS_EffApp*)
+Axiom MuAppAndEffAppShareArgument:
+ forall h'' env rho ef env' rho' f x ec' ee' ea aheap v eff facts1 aacts1 bacts1, 
+   (forall fheap h' bacts facts v' aacts, 
+      (h'', env, rho, ef) ⇓ (fheap, Cls (env', rho', Mu f x ec' ee'), facts) ->
+      (fheap, env, rho, ea) ⇓ (aheap, v, aacts) ->
+      (aheap, update_rec_E (f, Cls (env', rho', Mu f x ec' ee')) (x, v) env', rho', ec') ⇓ (h', v', bacts) ->
+      (h'', env, rho, Mu_App ef ea) ⇓ (h', v', Phi_Seq (Phi_Seq facts aacts)bacts)) -> 
+   (* above is the definition of the type constructor BS_Mu_App *)
+   (h'', env, rho, Eff_App ef ea) ⇓ (h'', eff, Phi_Seq (Phi_Seq facts1 aacts1) bacts1) ->
+   (aheap, update_rec_E (f, Cls (env', rho', Mu f x ec' ee')) (x, v) env', rho', ee') ⇓ (h'', eff, bacts1). 
+  
+(* Assuming that MuAppIncludesEffectShareArgument is a "specification", this prove the necessary goal *)
+Lemma EvaluationEffectFromEffApp:
+ forall h'' env rho ef env' rho' f x ec' ee' ea aheap v eff facts1 aacts1 bacts1,
+   (h'', env, rho, Eff_App ef ea) ⇓ (h'', eff, Phi_Seq (Phi_Seq facts1 aacts1) bacts1) ->
+   (aheap, update_rec_E (f, Cls (env', rho', Mu f x ec' ee')) (x, v) env', rho', ee') ⇓ (h'', eff, bacts1).
+Proof.
+  intros.
+  inversion H using MuAppAndEffAppShareArgument.
+  intros. econstructor; eauto.
+Qed. 
 
-Axiom EquivalenceUpToPermutations:
-  forall (h h' h_: Heap) env rho exp v p,
-    H.Equal h' h_ ->
-    H.Equal h h'  ->
-    (h, env, rho, exp) ⇓ (h', v, p) ->
-    h' = h_.
-
+(* Inside "BigStep" we still don't use "E.Equal" to pass around heaps. 
+   We need to resort to Coq equality when doing the proof for PairPar *)  
 Axiom ReadOnlyWalkSameHeap:
   forall acts_mu1 acts_mu2 h same_h,
     ReadOnlyPhi (Phi_Par acts_mu1 acts_mu2) ->
     (Phi_Par acts_mu1 acts_mu2, h) ==>* (Phi_Nil, same_h) ->
-    H.Equal h same_h.
+    (*H.Equal h same_h.*)
+    h = same_h.
 
-Axiom ReadOnlyTraceSameHeap :
-  forall h'' heap env rho exp eff phi,
-    ReadOnlyPhi phi ->
-    (h'', env, rho, exp) ⇓ (h'', eff, phi) ->
-    (heap, env, rho, exp) ⇓ (heap, eff, phi).
-
-Axiom EqualHeapsEqualFold :
-  forall heap_mu1 heap_mu0 heap_mu2 heap_mu3,
-    H.Equal heap_mu1 heap_mu0 ->
-    H.Equal heap_mu2 heap_mu3 ->
-    H.Equal (Functional_Map_Union_Heap heap_mu1 heap_mu2) 
-            (Functional_Map_Union_Heap heap_mu0 heap_mu3).
-
+(* Induction principle for TcHeap when we know that previous heaps are 
+   consistent and the new ones are non-overlapping. *)
 Axiom UnionTcHeap:
-  forall hp' heap_mu1 heap_mu2 sttym sttya,
-    H.Equal hp' (Functional_Map_Union_Heap heap_mu1 heap_mu2) ->
+  forall hp hp' ef1 ea1 ef2 ea2 theta1 theta2 v1 v2 acts_eff1 acts_eff2 env rho
+         heap heap_mu1 heap_mu2 heap_eff1 heap_eff2 sttym sttya acts_mu1 acts_mu2,
+    (heap, env, rho, Eff_App ef1 ea1) ⇓ (heap_eff1, Eff theta1, acts_eff1) ->
+    (heap, env, rho, Eff_App ef2 ea2) ⇓ (heap_eff2, Eff theta2, acts_eff2) ->
+    Disjointness theta1 theta2 /\ ~ Conflictness theta1 theta2 ->
+    (heap, env, rho, Mu_App ef1 ea1) ⇓ (heap_mu1, Num v1, acts_mu1) ->
+    (heap, env, rho, Mu_App ef2 ea2) ⇓ (heap_mu2, Num v2, acts_mu2) ->
+    (Phi_Par acts_mu1 acts_mu2, hp) ==>* (Phi_Nil, hp') ->
     TcHeap (heap_mu1, sttym) ->
     TcHeap (heap_mu2, sttya) ->
     TcHeap (hp', Functional_Map_Union sttya sttym).
@@ -55,7 +61,6 @@ Axiom UnionStoreTyping:
     ST.find (elt:=tau) l sttya = Some t' -> 
     ST.find (elt:=tau) l sttym = Some t' ->
     ST.find (elt:=tau) l (Functional_Map_Union sttya sttym) = Some t'.
-
 
 Axiom fold_subst_rgn_left_1:
   forall this1 k e this2 t x this1_is_bst,
