DeterminismExt.v
@@ -14,194 +14,772 @@ Require Import Coq.Arith.Compare_dec.
 Add LoadPath "." as Top0.
 Require Import Top0.Keys.
 Require Import Top0.Heap.
+Require Import Top0.Tactics.
 Require Import Top0.Environment.
 Require Import Top0.Definitions.
 Require Import Top0.CorrectnessLemmas.
 Require Import Top0.Determinism.
 Require Import Top0.TypeSystem.
-
+Require Import Top0.EffectSystem.
+Require Import Top0.Correctness.
 
 Axiom AllocAddressIsDeterministic:
   forall r0 l l0 heap,
     find_H (r0, l0) heap = find_H (r0, l) heap ->
     l = l0.
 
+Import EffectSoundness.
+Import TypeSoundness.
+
+Example PairParAux:
+  forall h'' heap_mu theta env v rho ef ea 
+         acts_eff acts_mu,
+   (h'', env, rho, Mu_App ef ea) ⇓ (heap_mu, Num v, acts_mu) ->
+   (h'', env, rho, Eff_App ef ea) ⇓ (h'', Eff theta, acts_eff) ->
+   forall stty ctxt rgns ty_e static_e,
+     TcHeap (h'', stty) ->
+     TcRho (rho, rgns) ->
+     TcEnv (stty, rho, env, ctxt) ->
+     TcExp (ctxt, rgns, Mu_App ef ea, ty_e, static_e) ->
+     acts_mu ⊑ theta /\ ReadOnlyPhi acts_eff.
+Proof.
+  intros.
+  inversion H4; subst.
+  assert (BackTriangle (ctxt, rgns, rho, Mu_App ef ea, Eff_App ef ea)) by (eapply H8). 
+  inversion H5; subst.
+  split.
+  - eapply Correctness_soundness_ext with (ea:=Mu_App ef ea); eauto using HFacts.Equal_refl.
+    assert (Epsilon_Phi_Soundness (fold_subst_eps rho static_ee, acts_eff)) 
+      by (eapply eff_sound; eauto). 
+    eapply ReadOnlyStaticImpliesReadOnlyPhi in H18; eauto.
+ -  assert (Epsilon_Phi_Soundness (fold_subst_eps rho static_ee, acts_eff)) 
+      by (eapply eff_sound; eauto). 
+    eapply ReadOnlyStaticImpliesReadOnlyPhi in H18; eauto.
+Qed.
+
+Theorem Dynamic_DetTrace :
+  forall heap rho env exp heap' val' phi',
+    forall stty ctxt rgns t static_eff,
+      TcHeap (heap, stty) ->
+      TcRho (rho, rgns) ->
+      TcEnv (stty, rho, env, ctxt) ->
+      TcExp (ctxt, rgns, exp, t, static_eff) ->
+      (heap, env, rho, exp) ⇓ (heap', val', phi') ->
+      Det_Trace phi'.
+Proof.
+  intros heap rho env exp heap' val' phi' stty ctxt rgns t static_eff HTcHeap HTcRho HTcEnv HTcExp HStep. 
+  generalize dependent stty.
+  generalize dependent rgns.
+  generalize dependent t.
+  generalize dependent ctxt.
+  generalize dependent static_eff.
+  dependent induction HStep; intros;
+  try (solve [repeat constructor; try (eapply IHHStep; reflexivity); try (eapply IHHStep1; reflexivity); try (eapply IHHStep2; reflexivity); try (eapply IHHStep3; reflexivity); try assumption]).
+  - constructor.  
+    + constructor. 
+      * inversion HTcExp; subst. eapply IHHStep1; eauto.
+      * inversion HTcExp; subst.
+        assert (clsTcVal : exists stty',  
+                             (forall l t', ST.find l stty = Some t' -> ST.find l stty' = Some t')
+                             /\ TcHeap (fheap, stty')
+                             /\ TcVal (stty', 
+                                       Cls (env', rho', Mu f x ec' ee'), 
+                                       subst_rho rho (Ty2_Arrow tya effc t effe Ty2_Effect))) 
+          by (eapply ty_sound; eauto).
+        destruct clsTcVal as [sttyb [Weakb [TcHeapb TcVal_cls]]]; eauto.
+        eapply IHHStep2; eauto using ext_stores__env.
+     +  inversion HTcExp; subst. 
+        assert (clsTcVal : exists stty',  
+                             (forall l t', ST.find l stty = Some t' -> ST.find l stty' = Some t')
+                             /\ TcHeap (fheap, stty')
+                             /\ TcVal (stty', 
+                                       Cls (env', rho', Mu f x ec' ee'), 
+                                       subst_rho rho (Ty2_Arrow tya effc t effe Ty2_Effect))) 
+          by (eapply ty_sound; eauto).
+        destruct clsTcVal as [sttyb [Weakb [TcHeapb TcVal_cls]]]; eauto.
+        assert (argTcVal : exists stty',
+                             (forall l t', ST.find l sttyb = Some t' -> ST.find l stty' = Some t')
+                             /\ TcHeap (aheap, stty')
+                             /\ TcVal (stty', v, subst_rho rho tya))
+          by (eapply ty_sound; eauto using update_env, ext_stores__env).
+        destruct argTcVal as [sttya [Weaka [TcHeapca TcVal_v']]]; eauto.
+        inversion TcVal_cls as [ | | | 
+                                 ? ? ? ? ? ? ? TcRho_rho' TcEnv_env' TcExp_abs [A B C D HSubst] 
+                                 | | |]; subst. 
+        inversion TcExp_abs as [ | | | 
+                                 ? ? ? ? ? ? ? ? ? ?  HBt_ec_ee TcExp_ec' TcExp_ee' 
+                                 | | | | | | | | | | | | | | | | | | | | |]; subst.
+        rewrite <- HSubst in TcVal_cls.
+        do 2 rewrite subst_rho_arrow in HSubst. 
+        inversion HSubst as [[H_tyx_tya A C D E]]; clear A C D E.
+        rewrite <- H_tyx_tya in TcVal_v'.
+        { eapply IHHStep3; eauto using ext_stores__env.
+          - apply update_env; simpl.  
+            + eapply ext_stores__env ; eauto. 
+              apply update_env.  
+              * eassumption.
+              * eapply ext_stores__val with (stty:=sttyb); eauto.
+            + eapply ext_stores__val with (stty:=sttya); eauto. }
+  - constructor; inversion HTcExp; subst.
+    + eapply IHHStep1; eauto.
+    + assert (clsTcVal : exists stty',  
+                          (forall l t', ST.find l stty = Some t' -> ST.find l stty' = Some t')
+                          /\ TcHeap (fheap, stty')
+                          /\ TcVal (stty', Cls (env', rho', Lambda x eb), 
+                                    subst_rho rho (Ty2_ForallRgn effr tyr))). 
+      eapply ty_sound;eauto. 
+      destruct clsTcVal as [sttyb [Weakb [TcHeapb TcVal_cls]]]; eauto.
+      
+      inversion TcVal_cls as [ | | | 
+                               ? ? ? ? ? ? ? TcRho_rho' TcEnv_env' TcExp_abs [A B C D HSubst] 
+                               | | |]; subst. 
+      inversion TcExp_abs as [ | | | |
+                               ? ? ? ? ? ? HNo HLc1 HLc2 HBt_eb HTExp_eb
+                               | | | | | | | | | | | | | | | | | | | |]; subst.
+      rewrite <- HSubst in TcVal_cls.
+      do 2 rewrite subst_rho_forallrgn in HSubst.
+      inversion HSubst as [[H_fold A]]; clear A.
+      
+      { eapply IHHStep2 with (heap:=fheap); eauto. 
+       - apply update_rho; auto. 
+       - eapply extended_rho; eauto. }   
+  - inversion HTcExp; subst. 
+    assert (clsTcVal : exists stty',  
+                         (forall l t', ST.find l stty = Some t' -> ST.find l stty' = Some t')
+                         /\ TcHeap (heap', stty')
+                         /\ TcVal (stty', 
+                                   Cls (env', rho', Mu f x ec' ee'), 
+                                   subst_rho rho (Ty2_Arrow tya effc tyc  effe Ty2_Effect))) 
+      by (eapply ty_sound; eauto).
+     destruct clsTcVal as [sttyb [Weakb [TcHeapb TcVal_cls]]]; eauto.
+     
+     assert (argTcVal : exists stty',
+                          (forall l t', ST.find l sttyb = Some t' -> ST.find l stty' = Some t')
+                          /\ TcHeap (heap', stty')
+                          /\ TcVal (stty', v', subst_rho rho tya))
+       by (eapply ty_sound; eauto using update_env, ext_stores__env).
+     destruct argTcVal as [sttya [Weaka [TcHeapa TcVal_v']]]; eauto.
+     
+     inversion TcVal_cls as [ | | | 
+                              ? ? ? ? ? ? ? TcRho_rho' TcEnv_env' TcExp_abs [A B C D HSubst] 
+                              | | |]; subst. 
+     inversion TcExp_abs as [ | | | 
+                              ? ? ? ? ? ? ? ? ? ? HBt_ec_ee TcExp_ec' TcExp_ee' 
+                              | | | | | | | | | | | | | | | | | | | | |]; subst.
+     rewrite <- HSubst in TcVal_cls.
+     do 2 rewrite subst_rho_arrow in HSubst. 
+     inversion HSubst as [[H_tyx_tya A C D E]]; clear A C D E.
+     rewrite <- H_tyx_tya in TcVal_v'.
+
+     constructor.
+     +  constructor.
+        * eapply IHHStep1; eauto using ext_stores__env.
+        * eapply IHHStep2; eauto using ext_stores__env.  
+     +  { eapply IHHStep3; eauto using ext_stores__env.
+          - apply update_env; simpl.  
+            + eapply ext_stores__env ; eauto. 
+              apply update_env.  
+              * eassumption.
+              * eapply ext_stores__val with (stty:=sttyb); eauto.
+            + eapply ext_stores__val with (stty:=sttya); eauto. }
+  - constructor; inversion HTcExp; subst.
+    + assert (HS1 : acts_mu1 ⊑ theta1 /\ ReadOnlyPhi acts_eff1). 
+      { eapply PairParAux; eauto. 
+        - inversion H5; subst.
+          assert (BackTriangle (ctxt, rgns, rho, Mu_App ef1 ea1, Eff_App ef1 ea1)) by (eapply H4).
+          inversion H1; subst.
+          
+          assert (Epsilon_Phi_Soundness (fold_subst_eps rho static_ee, acts_eff1)) 
+            by (eapply eff_sound; eauto). 
+          eapply ReadOnlyStaticImpliesReadOnlyPhi in H18; eauto.
+          assert (heap =heap_eff1). eapply ReadOnlyTracePreservesHeap_1; eauto. now subst. }
+
+      assert (HS2 : acts_mu2 ⊑ theta2 /\ ReadOnlyPhi acts_eff2).
+      { eapply PairParAux; eauto.  
+        - inversion H10; subst.
+          assert (BackTriangle (ctxt, rgns, rho, Mu_App ef2 ea2, Eff_App ef2 ea2)) by (eapply H4).
+          inversion H1; subst.
+          
+          assert (Epsilon_Phi_Soundness (fold_subst_eps rho static_ee, acts_eff2)) 
+            by (eapply eff_sound; eauto). 
+          eapply ReadOnlyStaticImpliesReadOnlyPhi in H18; eauto.
+          assert (heap =heap_eff2). eapply ReadOnlyTracePreservesHeap_1; eauto. subst; auto. }
+
+      destruct HS1, HS2. 
+      eapply Det_par_trace_from_readonly; try eassumption.
+    + eapply Det_trace_from_theta; try eassumption. 
+      * assert (HS1 : acts_mu1 ⊑ theta1 /\ ReadOnlyPhi acts_eff1).
+        { eapply PairParAux; eauto. 
+          - inversion H5; subst.
+            assert (BackTriangle (ctxt, rgns, rho, Mu_App ef1 ea1, Eff_App ef1 ea1)) by (eapply H4).
+            inversion H1; subst.
+            
+            assert (Epsilon_Phi_Soundness (fold_subst_eps rho static_ee, acts_eff1)) 
+              by (eapply eff_sound; eauto). 
+            eapply ReadOnlyStaticImpliesReadOnlyPhi in H18; eauto.
+            assert (heap =heap_eff1)
+              by (eapply ReadOnlyTracePreservesHeap_1; eauto).  
+            subst; eassumption. }
+        intuition.
+      *  assert (HS2 : acts_mu2 ⊑ theta2 /\ ReadOnlyPhi acts_eff2).
+         { eapply PairParAux; eauto.  
+           - inversion H10; subst.
+             assert (BackTriangle (ctxt, rgns, rho, Mu_App ef2 ea2, Eff_App ef2 ea2)) by (eapply H4).
+             inversion H1; subst.
+             
+             assert (Epsilon_Phi_Soundness (fold_subst_eps rho static_ee, acts_eff2)) 
+               by (eapply eff_sound; eauto). 
+             eapply ReadOnlyStaticImpliesReadOnlyPhi in H18; eauto.
+             assert (heap =heap_eff2) 
+               by (eapply ReadOnlyTracePreservesHeap_1; eauto). 
+             subst; eassumption. }
+         intuition.
+      * eapply IHHStep3; eauto.
+      * eapply IHHStep4; eauto.
+  -  constructor; inversion HTcExp; subst.
+     * eapply IHHStep1; eauto.
+     * assert (firstVal : exists stty',  
+                            (forall l t', ST.find l stty = Some t' -> ST.find l stty' = Some t')
+                            /\ TcHeap (cheap, stty')
+                            /\ TcVal (stty', 
+                                      Bit true, 
+                                      subst_rho rho Ty2_Boolean)). 
+       eapply ty_sound; eauto. 
+       destruct firstVal as [sttyb [Weakb [TcHeapb TcVal_bit]]]; eauto.
+       eapply IHHStep2; eauto using ext_stores__env.
+  - constructor; inversion HTcExp; subst.
+     * eapply IHHStep1; eauto.
+     * assert (firstVal : exists stty',  
+                            (forall l t', ST.find l stty = Some t' -> ST.find l stty' = Some t')
+                            /\ TcHeap (cheap, stty')
+                            /\ TcVal (stty', 
+                                      Bit false, 
+                                      subst_rho rho Ty2_Boolean)). 
+       eapply ty_sound; eauto. 
+       destruct firstVal as [sttyb [Weakb [TcHeapb TcVal_bit]]]; eauto.
+       eapply IHHStep2; eauto using ext_stores__env.
+  - constructor; inversion HTcExp; subst.
+    + eapply IHHStep; eauto.
+    + constructor.
+  - constructor; inversion HTcExp; subst.
+    + eapply IHHStep; eauto.
+    + constructor.
+  - constructor; inversion HTcExp; subst.
+    + constructor. 
+      * eapply IHHStep1; eauto.
+      * assert (argVal : exists stty',  
+                           (forall l t', ST.find l stty = Some t' -> ST.find l stty' = Some t')
+                           /\ TcHeap (heap'0, stty')
+                           /\ TcVal (stty', 
+                                     Loc (Rgn2_Const true false s) l, 
+                                     subst_rho rho ( Ty2_Ref (mk_rgn_type (Rgn2_Const true false s)) t0))). 
+        eapply ty_sound; eauto. 
+        destruct argVal as [sttyb [Weakb [TcHeapb TcVal_ea]]]; eauto.
+        eapply IHHStep2; eauto using ext_stores__env. 
+    + constructor.
+  - constructor; inversion HTcExp; subst.
+    + eapply IHHStep1; eauto.
+    + assert (argVal : exists stty',  
+                         (forall l t', ST.find l stty = Some t' -> ST.find l stty' = Some t')
+                         /\ TcHeap (lheap, stty')
+                         /\ TcVal (stty', 
+                                   Num va, 
+                                   subst_rho rho Ty2_Natural)). 
+      eapply ty_sound; eauto. 
+      destruct argVal as [sttyb [Weakb [TcHeapb TcVal_ea]]]; eauto.
+      eapply IHHStep2; eauto using ext_stores__env.
+  - constructor; inversion HTcExp; subst.
+    + eapply IHHStep1; eauto.
+    + assert (argVal : exists stty',  
+                         (forall l t', ST.find l stty = Some t' -> ST.find l stty' = Some t')
+                         /\ TcHeap (lheap, stty')
+                         /\ TcVal (stty', 
+                                   Num va, 
+                                   subst_rho rho Ty2_Natural)). 
+      eapply ty_sound; eauto. 
+      destruct argVal as [sttyb [Weakb [TcHeapb TcVal_ea]]]; eauto.
+      eapply IHHStep2; eauto using ext_stores__env.
+  - constructor; inversion HTcExp; subst.
+    + eapply IHHStep1; eauto.
+    + assert (argVal : exists stty',  
+                         (forall l t', ST.find l stty = Some t' -> ST.find l stty' = Some t')
+                         /\ TcHeap (lheap, stty')
+                         /\ TcVal (stty', 
+                                   Num va, 
+                                   subst_rho rho Ty2_Natural)). 
+      eapply ty_sound; eauto. 
+      destruct argVal as [sttyb [Weakb [TcHeapb TcVal_ea]]]; eauto.
+      eapply IHHStep2; eauto using ext_stores__env.
+  - constructor; inversion HTcExp; subst.
+    + eapply IHHStep1; eauto.
+    + assert (argVal : exists stty',  
+                         (forall l t', ST.find l stty = Some t' -> ST.find l stty' = Some t')
+                         /\ TcHeap (lheap, stty')
+                         /\ TcVal (stty', 
+                                   Num va, 
+                                   subst_rho rho Ty2_Natural)). 
+      eapply ty_sound; eauto. 
+      destruct argVal as [sttyb [Weakb [TcHeapb TcVal_ea]]]; eauto.
+      eapply IHHStep2; eauto using ext_stores__env.
+  - constructor; inversion HTcExp; subst.
+    + eapply IHHStep1; eauto.
+    + eapply IHHStep2; eauto.
+Qed.
+
+
 Theorem DynamicDeterminism_ext : 
   forall heap_a heap_b env rho exp heap1 heap2 val1 val2 acts1 acts2,
     H.Equal heap_a heap_b ->
     (heap_a, env, rho, exp) ⇓ (heap1, val1, acts1) ->
     (heap_b, env, rho, exp) ⇓ (heap2, val2, acts2) ->
-    H.Equal heap1 heap2 /\ val1 = val2 /\ acts1 = acts2.
+    forall stty ctxt rgns ty static,
+     TcHeap (heap_a, stty) ->
+     TcRho (rho, rgns) ->
+     TcEnv (stty, rho, env, ctxt) ->
+     TcExp (ctxt, rgns, exp, ty, static) ->
+     H.Equal heap1 heap2 /\ val1 = val2 /\ acts1 = acts2.
 Proof.
-  intros heap_a heap_b env rho exp heap1 heap2 val1 val2 acts1 acts2 Heq Dyn1. 
+  intros heap_a heap_b env rho exp heap1 heap2 val1 val2 acts1 acts2 Heq Dyn1.
   generalize dependent acts2; generalize dependent val2; generalize dependent heap2. 
-  generalize dependent heap_b. 
-  dependent induction Dyn1; intros heap_b Heq heap2 val2 acts2 Dyn2; inversion Dyn2; subst;
+  generalize dependent heap_b.
+  dependent induction Dyn1; 
+  intros heap_b Heq heap2 val2 acts2 Dyn2 stty ctxt rgns ty static HTcHeap HTcRho HTcEnv HTcExp;
+  inversion Dyn2; subst;
   try (solve [intuition]).
   - intuition. rewrite H in H1. inversion H1; subst. reflexivity.
-  - assert ( RH1 : H.Equal fheap fheap0 /\ Cls (env', rho', Mu f x ec' ee') = 
+  - inversion HTcExp as  [ | | | | | 
+                           ? ? ? ? ? ? ? ? ? ? HExp_ef HExp_ea 
+                           | | | | | | | | | | | | | | | | | | | ]; subst.
+    assert (clsTcVal : exists stty',  
+                         (forall l t', ST.find l stty = Some t' -> ST.find l stty' = Some t')
+                         /\ TcHeap (fheap, stty')
+                         /\ TcVal (stty', 
+                                   Cls (env', rho', Mu f x ec' ee'), 
+                                   subst_rho rho (Ty2_Arrow tya effc ty effe Ty2_Effect))) 
+      by (eapply ty_sound; eauto).
+    destruct clsTcVal as [sttyb [Weakb [TcHeapb TcVal_cls]]]; eauto.
+    
+    assert (argTcVal : exists stty',
+                         (forall l t', ST.find l sttyb = Some t' -> ST.find l stty' = Some t')
+                         /\ TcHeap (aheap, stty')
+                         /\ TcVal (stty', v, subst_rho rho tya))
+      by (eapply ty_sound; eauto using update_env, ext_stores__env).
+    destruct argTcVal as [sttya [Weaka [TcHeapa TcVal_v']]]; eauto.
+    
+    inversion TcVal_cls as [ | | | 
+                             ? ? ? ? ? ? ? TcRho_rho' TcEnv_env' TcExp_abs [A B C D HSubst] 
+                             | | |]; subst. 
+    inversion TcExp_abs as [ | | | 
+                             ? ? ? ? ? ? ? ? ? ? HBt_ec_ee TcExp_ec' TcExp_ee' 
+                             | | | | | | | | | | | | | | | | | | | | |]; subst.
+    rewrite <- HSubst in TcVal_cls.
+    do 2 rewrite subst_rho_arrow in HSubst. 
+    inversion HSubst as [[H_tyx_tya A C D E]]; clear A C D E.
+    rewrite <- H_tyx_tya in TcVal_v'.
+
+    assert ( RH1 : H.Equal fheap fheap0 /\ Cls (env', rho', Mu f x ec' ee') = 
                                            Cls (env'0, rho'0, Mu f0 x0 ec'0 ee'0) /\ facts = facts0 ).
     eapply IHDyn1_1; eauto. 
-    destruct RH1 as [h_eq_1 [v_eq_1 a_eq_1]]. inversion v_eq_1. subst.
-    assert ( RH2 : H.Equal aheap aheap0 /\ v = v0 /\ aacts = aacts0) by (eapply IHDyn1_2; eauto).
-    destruct RH2 as [h_eq_2 [v_eq_2 a_eq_2]]; subst. 
+    destruct RH1 as [h_eq_1 [v_eq_1 a_eq_1]]. inversion v_eq_1; subst.
+    assert ( RH2 : H.Equal aheap aheap0 /\ v = v0 /\ aacts = aacts0). 
+    
+    eapply IHDyn1_2; eauto using ext_stores__env.
+    destruct RH2 as [h_eq_2 [v_eq_2 a_eq_2]]; subst.
     
     assert ( RH3 : H.Equal heap1 heap2 /\ val1 = val2 /\ bacts = bacts0).
-    eapply IHDyn1_3; eauto. 
+    { eapply IHDyn1_3; eauto. 
+      - apply update_env; simpl.  
+        + eapply ext_stores__env; eauto.  
+          apply update_env; [eassumption | eapply ext_stores__val with (stty:=sttyb); eauto].
+        + eapply ext_stores__val with (stty:=sttya); eauto. }
     destruct RH3 as [h_eq_3 [v_eq_3 a_eq_3]]; subst.
     auto.
-  - assert ( RH1 : H.Equal fheap fheap0 /\  Cls (env', rho', Lambda x eb) =
+  -  inversion HTcExp as  [ | | | | | 
+                           |  ? ? ? ? ? ? ? HTcExp_er HTcRgn_w 
+                           | | | | | | | | | | | | | | | | | |]; subst.
+     assert (clsTcVal : exists stty',  
+                          (forall l t', ST.find l stty = Some t' -> ST.find l stty' = Some t')
+                          /\ TcHeap (fheap, stty')
+                          /\ TcVal (stty', Cls (env', rho', Lambda x eb), 
+                                    subst_rho rho (Ty2_ForallRgn effr tyr))). 
+     eapply ty_sound;eauto. 
+     destruct clsTcVal as [sttyb [Weakb [TcHeapb TcVal_cls]]]; eauto.
+     
+     inversion TcVal_cls as [ | | | 
+                              ? ? ? ? ? ? ? TcRho_rho' TcEnv_env' TcExp_abs [A B C D HSubst] 
+                              | | |]; subst. 
+     inversion TcExp_abs as [ | | | |
+                              ? ? ? ? ? ? HNo HLc1 HLc2 HBt_eb HTExp_eb
+                              | | | | | | | | | | | | | | | | | | | |]; subst.
+     rewrite <- HSubst in TcVal_cls.
+     do 2 rewrite subst_rho_forallrgn in HSubst.
+     inversion HSubst as [[H_fold A]]; clear A.
+     
+     
+     assert ( RH1 : H.Equal fheap fheap0 /\  Cls (env', rho', Lambda x eb) =
                                             Cls (env'0, rho'0, Lambda x0 eb0) /\ facts = facts0 ).
-    eapply IHDyn1_1; eauto.
-    destruct RH1 as [h_eq_1 [v_eq_1 a_eq_1]]. inversion v_eq_1. subst.
-    rewrite H in H9. inversion H9; subst.
+     eapply IHDyn1_1; eauto.
+     destruct RH1 as [h_eq_1 [v_eq_1 a_eq_1]]. inversion v_eq_1. subst.
+     rewrite H in H9. inversion H9; subst.
+    
+     assert ( RH2 : H.Equal heap1 heap2 /\ val1 = val2 /\ bacts = bacts0).
+     { eapply IHDyn1_2 with (heap_a:=fheap); eauto. 
+       - apply update_rho; auto.
+       - eapply extended_rho; eauto. }
+     
+     destruct RH2 as [h_eq_2 [v_eq_2 a_eq_2]]. subst.
+     intuition.    
+  -  inversion HTcExp as  [ | | | | | ? ? ? ? ? ? ? ? ? ? ? HExp_ef HExp_ea 
+                            | | | 
+                            ? ? ? ? ? ? ? ? ? ? ? ? ? ? HExp_mu1 HExp_mu2 HExp_eff1 HExp_eff2 
+                            | | | | | | | | | | | | | | | | ]; subst.
+     assert (clsTcVal : exists stty',  
+                          (forall l t', ST.find l stty = Some t' -> ST.find l stty' = Some t')
+                          /\ TcHeap (heap1, stty')
+                          /\ TcVal (stty', 
+                                    Cls (env', rho', Mu f x ec' ee'), 
+                                    subst_rho rho (Ty2_Arrow tya effc tyc  effe Ty2_Effect))) 
+       by (eapply ty_sound; eauto).
+     destruct clsTcVal as [sttyb [Weakb [TcHeapb TcVal_cls]]]; eauto.
+     
+     assert (argTcVal : exists stty',
+                          (forall l t', ST.find l sttyb = Some t' -> ST.find l stty' = Some t')
+                          /\ TcHeap (heap1, stty')
+                          /\ TcVal (stty', v', subst_rho rho tya))
+       by (eapply ty_sound; eauto using update_env, ext_stores__env).
+     destruct argTcVal as [sttya [Weaka [TcHeapa TcVal_v']]]; eauto.
+     
+     inversion TcVal_cls as [ | | | 
+                              ? ? ? ? ? ? ? TcRho_rho' TcEnv_env' TcExp_abs [A B C D HSubst] 
+                              | | |]; subst. 
+     inversion TcExp_abs as [ | | | 
+                              ? ? ? ? ? ? ? ? ? ? HBt_ec_ee TcExp_ec' TcExp_ee' 
+                              | | | | | | | | | | | | | | | | | | | | |]; subst. 
+     rewrite <- HSubst in TcVal_cls. 
+     do 2 rewrite subst_rho_arrow in HSubst.
+     inversion HSubst as [[H_tyx_tya A C D E]]; clear A C D E.
+     rewrite <- H_tyx_tya in TcVal_v'.
+     
+     assert ( RH1 : H.Equal heap1 heap2 /\  Cls (env', rho', Mu f x ec' ee') =
+                                            Cls (env'0, rho'0, Mu f0 x0 ec'0 ee'0) /\ facts = facts0 ).
+     eapply IHDyn1_1; eauto using ext_stores__env.
+     destruct RH1 as [h_eq_1 [v_eq_1 a_eq_1]]. inversion v_eq_1. subst.
+     
+     assert ( RH2 : H.Equal heap1 heap2 /\  v' = v'0 /\ aacts = aacts0 ).
+     eapply IHDyn1_2;  eauto using ext_stores__env.
+     destruct RH2 as [h_eq_2 [v_eq_2 a_eq_2]]. inversion v_eq_2. subst.
+     
+     assert ( RH3 : H.Equal heap1 heap2 /\  val1 = val2 /\ bacts = bacts0 ).  
+     { eapply IHDyn1_3; eauto.
+       - apply update_env; simpl.  
+          + eapply ext_stores__env ; eauto. 
+                  apply update_env.  
+                  * eassumption.
+                  * eapply ext_stores__val with (stty:=sttyb); eauto.
+                + eapply ext_stores__val with (stty:=sttya); eauto. }
+     destruct RH3 as [h_eq_3 [v_eq_3 a_eq_3]]. inversion v_eq_3. subst.
+     intuition.
+  - inversion HTcExp as  [ | | | | | ? ? ? ? ? ? ? ? ? ? HExp_ef HExp_ea 
+                           | | | 
+                           ? ? ? ? ? ? ? ? ? ? ? ? ? ? HExp_mu1 HExp_mu2 HExp_eff1 HExp_eff2 
+                           | | | | | | | | | | | | | | | | ]; subst.
+    
+    inversion HExp_mu1; subst.
+    assert (BackTriangle (ctxt, rgns, rho, Mu_App ef1 ea1, Eff_App ef1 ea1)) by (eapply H4).
+    inversion HExp_mu2; subst.
+    assert (BackTriangle (ctxt, rgns, rho, Mu_App ef2 ea2, Eff_App ef2 ea2)) by (eapply H6).
+ 
+    inversion H1; inversion H2; subst.
+          
+    assert (Epsilon_Phi_Soundness (fold_subst_eps rho static_ee, acts_eff1)) 
+      by (eapply eff_sound; eauto). 
+    assert (Epsilon_Phi_Soundness (fold_subst_eps rho static_ee0,acts_eff2)) 
+      by (eapply eff_sound; eauto). 
+    assert (Epsilon_Phi_Soundness (fold_subst_eps rho static_ee0, acts_eff3)) 
+      by (eapply eff_sound; eauto; eapply EqualHeaps; eauto).
+    assert (Epsilon_Phi_Soundness (fold_subst_eps rho static_ee, acts_eff0)) 
+      by (eapply eff_sound; eauto; eapply EqualHeaps; eauto).
+ 
+    assert (ReadOnlyPhi acts_eff1 ) 
+      by (eapply ReadOnlyStaticImpliesReadOnlyPhi with(eps:=fold_subst_eps rho static_ee); eauto).
+    assert (ReadOnlyPhi acts_eff2 ) 
+      by (eapply ReadOnlyStaticImpliesReadOnlyPhi with(eps:=fold_subst_eps rho static_ee0); eauto).
+    assert (ReadOnlyPhi acts_eff0 ) 
+      by (eapply ReadOnlyStaticImpliesReadOnlyPhi with(eps:=fold_subst_eps rho static_ee); eauto).
+    assert (ReadOnlyPhi acts_eff3 ) 
+      by (eapply ReadOnlyStaticImpliesReadOnlyPhi with(eps:=fold_subst_eps rho static_ee0); eauto).
 
-    assert ( RH2 : H.Equal heap1 heap2 /\ val1 = val2 /\ bacts = bacts0).
-    eapply IHDyn1_2; eauto.
+    assert (HR1 : H.Equal heap_a heap_b /\ Eff theta1 = Eff theta0 /\ acts_eff1 = acts_eff0).   
+    { eapply IHDyn1_1; eauto. 
+      - assert (heap_a =heap_eff1) by (eapply ReadOnlyTracePreservesHeap_1; eauto; subst; eassumption).
+        rewrite H34; reflexivity.
+      - assert (heap_b =heap_eff0) by (eapply ReadOnlyTracePreservesHeap_1; eauto; subst; eassumption).
+        rewrite H34. rewrite H34 in H7. assumption. } 
+    destruct HR1 as [h_eq_1 [v_eq_1 a_eq_1]]. inversion v_eq_1.  subst.
+    
+    assert (HR2 : H.Equal heap_eff2 heap_eff3 /\ Eff theta2 = Eff theta3 /\ acts_eff2 = acts_eff3). 
+    eapply IHDyn1_2; eauto.    
+    destruct HR2 as [h_eq_2 [v_eq_2 a_eq_2]]. inversion v_eq_2. subst.
+    
+    assert (HR3 : H.Equal heap_mu1 heap_mu0 /\ Num v1 = Num v0 /\ acts_mu1 = acts_mu0).  
+    eapply IHDyn1_3; eauto.
+    inversion HR3 as [h_eq_3 [v_eq_3 a_eq_3]]. inversion v_eq_3.
+    
+    assert (HR4 : H.Equal heap_mu2 heap_mu3 /\ Num v2 = Num v3 /\ acts_mu2 = acts_mu3).  
+    eapply IHDyn1_4; eauto.
+    inversion HR4 as [h_eq_4 [v_eq_4 a_eq_4]]. inversion v_eq_4.
+
+    assert (HS1 : acts_mu0 ⊑ theta0 ). 
+    { eapply PairParAux; eauto.
+      - assert (heap_b =heap_eff0) by (eapply ReadOnlyTracePreservesHeap_1; eauto; subst; eassumption).
+         rewrite H34. rewrite H34 in H7. eassumption.
+      - eapply EqualHeaps; eauto.  
+    } inversion HExp_mu1.
+    
+    assert (HS2 : acts_mu3 ⊑ theta3 ).
+    { eapply PairParAux; eauto.  
+      - assert (heap_b =heap_eff3) by (eapply ReadOnlyTracePreservesHeap_1; eauto; subst; eassumption).
+        rewrite H56. rewrite H56 in H12. eassumption.
+      - eapply EqualHeaps; eauto. 
+    } inversion HExp_mu2. 
+    
+    intuition. 
+    eapply unique_heap_new with  (heapa := heap_a) (heapb := heap_b) (theta1:=theta0) (theta2:=theta3); eauto.
+    * assert (Det_Trace (Phi_Par acts_mu0 acts_mu3)).
+      subst. eapply Det_trace_from_theta; eauto; 
+      [ eapply Dynamic_DetTrace in Dyn1_3 | eapply Dynamic_DetTrace in Dyn1_4]; eassumption.  
+      now inversion H70.
+    * assert (Det_Trace (Phi_Par acts_mu0 acts_mu3))
+        by (subst; eapply Det_trace_from_theta; eauto; 
+            [ eapply Dynamic_DetTrace in Dyn1_3 | eapply Dynamic_DetTrace in Dyn1_4]; eassumption).
+      now inversion H70.
+    * rewrite <- H72. rewrite <- H73. eassumption.
+    * rewrite <- H72. rewrite <- H73. reflexivity.
+  - inversion HTcExp; subst;
+    assert ( RH1 : H.Equal cheap cheap0 /\  Bit true = Bit true /\ cacts = cacts0 ).
+    eapply IHDyn1_1; eauto.
+    destruct RH1 as [h_eq_1 [v_eq_1 a_eq_1]]. subst.
+    assert ( RH2 : H.Equal heap1 heap2 /\ val1 = val2 /\ tacts = tacts0 ).
+    
+    assert (firstVal : exists stty',  
+                         (forall l t', ST.find l stty = Some t' -> ST.find l stty' = Some t')
+                         /\ TcHeap (cheap, stty')
+                         /\ TcVal (stty', 
+                                   Bit true, 
+                                   subst_rho rho Ty2_Boolean)). 
+    eapply ty_sound; eauto. 
+    destruct firstVal as [sttyb [Weakb [TcHeapb TcVal_bit]]]; eauto.
+
+    eapply IHDyn1_2 with (stty:=sttyb); eauto using ext_stores__env. 
     destruct RH2 as [h_eq_2 [v_eq_2 a_eq_2]]. subst.
     intuition.
-  - assert ( RH1 : H.Equal heap1 heap2 /\  Cls (env', rho', Mu f x ec' ee') =
-                                           Cls (env'0, rho'0, Mu f0 x0 ec'0 ee'0) /\ facts = facts0 ).
+  - inversion HTcExp; subst;
+    assert ( RH1: H.Equal cheap cheap0 /\ Bit true = Bit false /\ cacts = cacts0). 
     eapply IHDyn1_1; eauto.
-    destruct RH1 as [h_eq_1 [v_eq_1 a_eq_1]]. inversion v_eq_1. subst.
+    destruct RH1 as [? [D ?]]. discriminate D.
+  - inversion HTcExp; subst.
+    assert ( RH1: H.Equal cheap cheap0 /\ Bit false = Bit true /\ cacts = cacts0). 
+    eapply IHDyn1_1; eauto.
+    destruct RH1 as [? [D ?]]. discriminate D.
+  - inversion HTcExp; subst.
+    assert ( RH1 : H.Equal cheap cheap0 /\  Bit false = Bit false /\ cacts = cacts0 ).
+    eapply IHDyn1_1; eauto.
+    destruct RH1 as [h_eq_1 [v_eq_1 a_eq_1]]. subst.
+
+    assert (firstVal : exists stty',  
+                         (forall l t', ST.find l stty = Some t' -> ST.find l stty' = Some t')
+                         /\ TcHeap (cheap, stty')
+                         /\ TcVal (stty', 
+                                   Bit false, 
+                                   subst_rho rho Ty2_Boolean)). 
+    eapply ty_sound; eauto. 
+    destruct firstVal as [sttyb [Weakb [TcHeapb TcVal_bit]]]; eauto.
+
+    assert ( RH2 : H.Equal heap1 heap2 /\ val1 = val2 /\ facts = facts0 ).
     
-    assert ( RH2 : H.Equal heap1 heap2 /\  v' = v'0 /\ aacts = aacts0 ).
+    eapply IHDyn1_2  with (stty:=sttyb); eauto using ext_stores__env. 
+    destruct RH2 as [h_eq_2 [v_eq_2 a_eq_2]]. subst.
+    intuition.
+  - inversion HTcExp; subst.
+    assert ( RH1 : H.Equal heap' heap'0 /\  v = v0 /\ vacts = vacts0 ).
+    eapply IHDyn1; eauto. 
+    destruct RH1 as [h_eq_1 [v_eq_1 a_eq_1]]. 
+    inversion v_eq_1.
+    rewrite H in H10. inversion H10; subst.
+    assert (HFind : forall k, find_H k heap' = find_H k heap'0)
+      by (unfold find_H, update_H; simpl; intro; apply HFacts.find_m; intuition).
+    rewrite HFind in H0.
+    rewrite <- H11 in H0; inversion H0; subst.
+    apply AllocAddressIsDeterministic in H0; subst.
+    intuition.
+    unfold update_H; simpl. apply HMapP.add_m; auto.
+  - inversion HTcExp; subst.
+    assert ( RH1 : H.Equal heap1 heap2 /\  
+                   Loc (Rgn2_Const true false s) l = Loc (Rgn2_Const true false s) l0 /\ 
+                   aacts = aacts0 ).
+    eapply IHDyn1; eauto. 
+    destruct RH1 as [h_eq_1 [v_eq_1 a_eq_1]]. 
+    inversion v_eq_1.
+    rewrite H in H10. inversion H10; subst.
+    assert (H5 : forall k, find_H k heap1 = find_H k heap2)
+      by (unfold find_H, update_H; simpl; intro; apply HFacts.find_m; intuition).
+    rewrite H5 in H0.
+    rewrite H11 in H0; inversion H0; subst.
+    intuition.
+  - inversion HTcExp; subst.
+    assert ( RH1 : H.Equal heap' heap'0 /\  
+                   Loc (Rgn2_Const true false s) l = Loc (Rgn2_Const true false s) l0 /\ 
+                   aacts = aacts0 ). 
+    eapply IHDyn1_1; eauto. 
+    destruct RH1 as [h_eq_1 [v_eq_1 a_eq_1]]. inversion v_eq_1.
+    
+    assert (argVal : exists stty',  
+                       (forall l t', ST.find l stty = Some t' -> ST.find l stty' = Some t')
+                       /\ TcHeap (heap', stty')
+                       /\ TcVal (stty', 
+                                 Loc (Rgn2_Const true false s) l, 
+                                 subst_rho rho ( Ty2_Ref (mk_rgn_type (Rgn2_Const true false s)) t))). 
+    eapply ty_sound; eauto. 
+    destruct argVal as [sttyb [Weakb [TcHeapb TcVal_ea]]]; eauto.
+
+    assert ( RH2 : H.Equal heap'' heap''0 /\ v = v0 /\ vacts = vacts0 ). 
+    eapply IHDyn1_2 with  (stty:=sttyb); eauto using ext_stores__env.
+    destruct RH2 as [h_eq_2 [v_eq_2 a_eq_2]]. inversion v_eq_2.
+    rewrite H in H11; inversion H11; subst. 
+    intuition.
+    unfold update_H; simpl. apply HMapP.add_m; auto. 
+  - inversion HTcExp; subst.
+    assert ( RH1 : H.Equal lheap lheap0 /\  Num va = Num va0 /\ lacts = lacts0 ). 
+    eapply IHDyn1_1; eauto.  
+    destruct RH1 as [h_eq_1 [v_eq_1 a_eq_1]]. inversion v_eq_1. subst.
+    assert ( RH2 : H.Equal heap1 heap2 /\ Num vb = Num vb0 /\ racts = racts0 ).  
+    
+    assert (argVal : exists stty',  
+                       (forall l t', ST.find l stty = Some t' -> ST.find l stty' = Some t')
+                       /\ TcHeap (lheap, stty')
+                       /\ TcVal (stty', 
+                                 Num va0, 
+                                 subst_rho rho Ty2_Natural)). 
+    eapply ty_sound; eauto. 
+    destruct argVal as [sttyb [Weakb [TcHeapb TcVal_ea]]]; eauto.
+    
+    eapply IHDyn1_2;  eauto using ext_stores__env.
+    destruct RH2 as [h_eq_2 [v_eq_2 a_eq_2]]. inversion v_eq_2. subst.
+    intuition.
+  - inversion HTcExp; subst.
+    assert ( RH1 : H.Equal lheap lheap0 /\  Num va = Num va0 /\ lacts = lacts0 ). 
+    eapply IHDyn1_1; eauto.  
+    destruct RH1 as [h_eq_1 [v_eq_1 a_eq_1]]. inversion v_eq_1. subst.
+    assert ( RH2 : H.Equal heap1 heap2 /\ Num vb = Num vb0 /\ racts = racts0 ).  
+    
+    assert (argVal : exists stty',  
+                       (forall l t', ST.find l stty = Some t' -> ST.find l stty' = Some t')
+                       /\ TcHeap (lheap, stty')
+                       /\ TcVal (stty', 
+                                 Num va0, 
+                                 subst_rho rho Ty2_Natural)). 
+    eapply ty_sound; eauto. 
+    destruct argVal as [sttyb [Weakb [TcHeapb TcVal_ea]]]; eauto.
+    
+    eapply IHDyn1_2;  eauto using ext_stores__env.
+    destruct RH2 as [h_eq_2 [v_eq_2 a_eq_2]]. inversion v_eq_2. subst.
+    intuition.  
+  - inversion HTcExp; subst.
+    assert ( RH1 : H.Equal lheap lheap0 /\  Num va = Num va0 /\ lacts = lacts0 ). 
+    eapply IHDyn1_1; eauto.  
+    destruct RH1 as [h_eq_1 [v_eq_1 a_eq_1]]. inversion v_eq_1. subst.
+    assert ( RH2 : H.Equal heap1 heap2 /\ Num vb = Num vb0 /\ racts = racts0 ).  
+    
+    assert (argVal : exists stty',  
+                       (forall l t', ST.find l stty = Some t' -> ST.find l stty' = Some t')
+                       /\ TcHeap (lheap, stty')
+                       /\ TcVal (stty', 
+                                 Num va0, 
+                                 subst_rho rho Ty2_Natural)). 
+    eapply ty_sound; eauto. 
+    destruct argVal as [sttyb [Weakb [TcHeapb TcVal_ea]]]; eauto.
+    
+    eapply IHDyn1_2;  eauto using ext_stores__env.
+    destruct RH2 as [h_eq_2 [v_eq_2 a_eq_2]]. inversion v_eq_2. subst.
+    intuition.
+  - inversion HTcExp; subst.
+    assert ( RH1 : H.Equal lheap lheap0 /\  Num va = Num va0 /\ lacts = lacts0 ). 
+    eapply IHDyn1_1; eauto.  
+    destruct RH1 as [h_eq_1 [v_eq_1 a_eq_1]]. inversion v_eq_1. subst.
+    assert ( RH2 : H.Equal heap1 heap2 /\ Num vb = Num vb0 /\ racts = racts0 ).  
+    
+    assert (argVal : exists stty',  
+                       (forall l t', ST.find l stty = Some t' -> ST.find l stty' = Some t')
+                       /\ TcHeap (lheap, stty')
+                       /\ TcVal (stty', 
+                                 Num va0, 
+                                 subst_rho rho Ty2_Natural)). 
+    eapply ty_sound; eauto. 
+    destruct argVal as [sttyb [Weakb [TcHeapb TcVal_ea]]]; eauto.
+    
+    eapply IHDyn1_2;  eauto using ext_stores__env.
+    destruct RH2 as [h_eq_2 [v_eq_2 a_eq_2]]. inversion v_eq_2. subst.
+    intuition.
+  - rewrite H in H1. inversion H1; subst. 
+    intuition.
+  - rewrite H in H1. inversion H1; subst. 
+    intuition.
+  - rewrite H in H1. inversion H1; subst. 
+    intuition.  
+  - inversion HTcExp; subst.
+    assert ( RH1 : H.Equal heap1 heap2 /\  Loc (Rgn2_Const true false r) l = 
+                                           Loc (Rgn2_Const true false r0) l0 /\ Phi_Nil = Phi_Nil ). 
+    eapply IHDyn1; eauto.  
+    destruct RH1 as [h_eq_1 [v_eq_1 a_eq_1]]. inversion v_eq_1. subst.
+    intuition.
+  - inversion HTcExp; subst.
+    assert ( RH1 : H.Equal heap1 heap2 /\  Loc (Rgn2_Const true false r) l = 
+                                           Loc (Rgn2_Const true false r0) l0 /\ Phi_Nil = Phi_Nil ). 
+    eapply IHDyn1; eauto.  
+    destruct RH1 as [h_eq_1 [v_eq_1 a_eq_1]]. inversion v_eq_1. subst.
+    intuition. 
+  - inversion HTcExp; subst.
+    assert ( RH1 : H.Equal heap1 heap2 /\  Eff effa = Eff effa0 /\ phia = phia0 ). 
+    eapply IHDyn1_1; eauto.  
+    destruct RH1 as [h_eq_1 [v_eq_1 a_eq_1]]. inversion v_eq_1. subst.
+    assert ( RH2 : H.Equal heap1 heap2 /\ Eff effb = Eff effb0 /\ phib = phib0 ). 
     eapply IHDyn1_2; eauto.
     destruct RH2 as [h_eq_2 [v_eq_2 a_eq_2]]. inversion v_eq_2. subst.
-
-    assert ( RH3 : H.Equal heap1 heap2 /\  val1 = val2 /\ bacts = bacts0 ).
-    eapply IHDyn1_3; eauto.
-    destruct RH3 as [h_eq_3 [v_eq_3 a_eq_3]]. inversion v_eq_3. subst.
     intuition.
-  - assert (HR1 : H.Equal heap_a heap_b /\ Eff theta1 = Eff theta0 /\ acts_eff1 = acts_eff0) 
-      by (eapply IHDyn1_1; eauto).
-    destruct HR1 as [h_eq_1 [v_eq_1 a_eq_1]]. inversion v_eq_1. subst.
-    assert (HR2 : H.Equal heap_a heap_b /\ Eff theta2 = Eff theta3 /\ acts_eff2 = acts_eff3) 
-      by (eapply IHDyn1_2; eauto).
-    destruct HR2 as [h_eq_2 [v_eq_2 a_eq_2]]. inversion v_eq_2. subst.
-    assert (HR3 : H.Equal heap_mu1 heap_mu0 /\ Num v1 = Num v0 /\ acts_mu1 = acts_mu0)  
-      by (eapply IHDyn1_3; eauto). 
-    inversion HR3 as [h_eq_3 [v_eq_3 a_eq_3]]. inversion v_eq_3. 
-    assert (HR4 : H.Equal heap_mu2 heap_mu3 /\ Num v2 = Num v3 /\ acts_mu2 = acts_mu3)  
-      by (eapply IHDyn1_4; eauto).  
-    inversion HR4 as [h_eq_4 [v_eq_4 a_eq_4]]. inversion v_eq_4. subst.
-    intuition. 
-    eapply unique_heap_new with (heapa := heap_a) (heapb := heap_b) (theta1:=theta0) (theta2:=theta3). 
-    + eauto. (* from correctness *)
-    + eauto. (* from correctness *) 
-    + eauto. (* from correctness *) 
-    + assert (Det_Trace (Phi_Par acts_mu0 acts_mu3))
-        by (eapply Det_trace_from_theta; eauto; 
-            [ apply Dynamic_DetTrace in Dyn1_3 | apply Dynamic_DetTrace in Dyn1_4]; assumption).
-      now inversion H12.
-    + assert (Det_Trace (Phi_Par acts_mu0 acts_mu3))
-        by (eapply Det_trace_from_theta; eauto; 
-            [ apply Dynamic_DetTrace in Dyn1_3 | apply Dynamic_DetTrace in Dyn1_4]; assumption).
-      now inversion H12.
-    + assumption.
-    + assumption.
-    + assumption.  
-  -  assert ( RH1 : H.Equal cheap cheap0 /\  Bit true = Bit true /\ cacts = cacts0 ).
-     eapply IHDyn1_1; eauto.
-     destruct RH1 as [h_eq_1 [v_eq_1 a_eq_1]]. subst.
-     assert ( RH2 : H.Equal heap1 heap2 /\ val1 = val2 /\ tacts = tacts0 ).
-     eapply IHDyn1_2; eauto.
-     destruct RH2 as [h_eq_2 [v_eq_2 a_eq_2]]. subst.
-     intuition.
-   - assert ( RH1: H.Equal cheap cheap0 /\ Bit true = Bit false /\ cacts = cacts0). 
-     eapply IHDyn1_1; eauto.
-     destruct RH1 as [? [D ?]]. discriminate D.
-   - assert ( RH1: H.Equal cheap cheap0 /\ Bit false = Bit true /\ cacts = cacts0). 
-     eapply IHDyn1_1; eauto.
-     destruct RH1 as [? [D ?]]. discriminate D.
-   - assert ( RH1 : H.Equal cheap cheap0 /\  Bit false = Bit false /\ cacts = cacts0 ).
-     eapply IHDyn1_1; eauto.
-     destruct RH1 as [h_eq_1 [v_eq_1 a_eq_1]]. subst.
-     assert ( RH2 : H.Equal heap1 heap2 /\ val1 = val2 /\ facts = facts0 ).
-     eapply IHDyn1_2; eauto.
-     destruct RH2 as [h_eq_2 [v_eq_2 a_eq_2]]. subst.
-     intuition.
-   - assert ( RH1 : H.Equal heap' heap'0 /\  v = v0 /\ vacts = vacts0 ).
-     eapply IHDyn1; eauto. 
-     destruct RH1 as [h_eq_1 [v_eq_1 a_eq_1]]. subst.
-     rewrite H in H10. inversion H10; subst.
-     assert (H5 : forall k, find_H k heap' = find_H k heap'0)
-       by (unfold find_H, update_H; simpl; intro; apply HFacts.find_m; intuition).
-     rewrite H5 in H0. 
-     rewrite <-H11 in H0. symmetry in H0.
-     apply AllocAddressIsDeterministic in H0; subst.
-     intuition.
-     unfold update_H; simpl. apply HMapP.add_m; auto.
-   - assert ( RH1 : H.Equal heap1 heap2 /\  Loc w l = Loc w l0 /\ aacts = aacts0 ).
-     eapply IHDyn1; eauto. 
-     destruct RH1 as [h_eq_1 [v_eq_1 a_eq_1]]. 
-     inversion v_eq_1.
-     rewrite H in H10. inversion H10; subst.
-     assert (H5 : forall k, find_H k heap1 = find_H k heap2)
-       by (unfold find_H, update_H; simpl; intro; apply HFacts.find_m; intuition).
-     rewrite H5 in H0.
-     rewrite H11 in H0; inversion H0; subst.
-     intuition.
-   - assert ( RH1 : H.Equal heap' heap'0 /\  Loc w l = Loc w l0 /\ aacts = aacts0 ). 
-     eapply IHDyn1_1; eauto. 
-     destruct RH1 as [h_eq_1 [v_eq_1 a_eq_1]]. inversion v_eq_1.
-     assert ( RH2 : H.Equal heap'' heap''0 /\ v = v0 /\ vacts = vacts0 ). 
-     eapply IHDyn1_2; eauto. 
-     destruct RH2 as [h_eq_2 [v_eq_2 a_eq_2]]. inversion v_eq_2.
-     rewrite H in H11; inversion H11; subst. 
-     intuition.
-     unfold update_H; simpl. apply HMapP.add_m; auto. 
-   - assert ( RH1 : H.Equal lheap lheap0 /\  Num va = Num va0 /\ lacts = lacts0 ). 
-     eapply IHDyn1_1; eauto.  
-     destruct RH1 as [h_eq_1 [v_eq_1 a_eq_1]]. inversion v_eq_1. subst.
-     assert ( RH2 : H.Equal heap1 heap2 /\ Num vb = Num vb0 /\ racts = racts0 ). 
-     eapply IHDyn1_2; eauto.
-     destruct RH2 as [h_eq_2 [v_eq_2 a_eq_2]]. inversion v_eq_2. subst.
-     intuition.
-   - assert ( RH1 : H.Equal lheap lheap0 /\  Num va = Num va0 /\ lacts = lacts0 ). 
-     eapply IHDyn1_1; eauto.  
-     destruct RH1 as [h_eq_1 [v_eq_1 a_eq_1]]. inversion v_eq_1. subst.
-     assert ( RH2 : H.Equal heap1 heap2 /\ Num vb = Num vb0 /\ racts = racts0 ). 
-     eapply IHDyn1_2; eauto.
-     destruct RH2 as [h_eq_2 [v_eq_2 a_eq_2]]. inversion v_eq_2. subst.
-     intuition.
-   - assert ( RH1 : H.Equal lheap lheap0 /\  Num va = Num va0 /\ lacts = lacts0 ). 
-     eapply IHDyn1_1; eauto.  
-     destruct RH1 as [h_eq_1 [v_eq_1 a_eq_1]]. inversion v_eq_1. subst.
-     assert ( RH2 : H.Equal heap1 heap2 /\ Num vb = Num vb0 /\ racts = racts0 ). 
-     eapply IHDyn1_2; eauto.
-     destruct RH2 as [h_eq_2 [v_eq_2 a_eq_2]]. inversion v_eq_2. subst.
-     intuition.
-   - assert ( RH1 : H.Equal lheap lheap0 /\  Num va = Num va0 /\ lacts = lacts0 ). 
-     eapply IHDyn1_1; eauto.  
-     destruct RH1 as [h_eq_1 [v_eq_1 a_eq_1]]. inversion v_eq_1. subst.
-     assert ( RH2 : H.Equal heap1 heap2 /\ Num vb = Num vb0 /\ racts = racts0 ). 
-     eapply IHDyn1_2; eauto.
-     destruct RH2 as [h_eq_2 [v_eq_2 a_eq_2]]. inversion v_eq_2. subst.
-     intuition.
-   - rewrite H in H1. inversion H1; subst. 
-     intuition.
-   - rewrite H in H1. inversion H1; subst. 
-     intuition.
-   - rewrite H in H1. inversion H1; subst. 
-     intuition.
-   - assert ( RH1 : H.Equal heap1 heap2 /\  Loc (Rgn2_Const true false r) l = 
-                                            Loc (Rgn2_Const true false r0) l0 /\ Phi_Nil = Phi_Nil ). 
-     eapply IHDyn1; eauto.  
-     destruct RH1 as [h_eq_1 [v_eq_1 a_eq_1]]. inversion v_eq_1. subst.
-     intuition.
-   - assert ( RH1 : H.Equal heap1 heap2 /\  Loc (Rgn2_Const true false r) l = 
-                                            Loc (Rgn2_Const true false r0) l0 /\ Phi_Nil = Phi_Nil ). 
-     eapply IHDyn1; eauto.  
-     destruct RH1 as [h_eq_1 [v_eq_1 a_eq_1]]. inversion v_eq_1. subst.
-     intuition. 
-   - assert ( RH1 : H.Equal heap1 heap2 /\  Eff effa = Eff effa0 /\ phia = phia0 ). 
-     eapply IHDyn1_1; eauto.  
-     destruct RH1 as [h_eq_1 [v_eq_1 a_eq_1]]. inversion v_eq_1. subst.
-     assert ( RH2 : H.Equal heap1 heap2 /\ Eff effb = Eff effb0 /\ phib = phib0 ). 
-     eapply IHDyn1_2; eauto.
-     destruct RH2 as [h_eq_2 [v_eq_2 a_eq_2]]. inversion v_eq_2. subst.
-     intuition.
 Qed.
 
+Require Import Top0.Heap.
 
+Theorem DynamicDeterminism : 
+  forall env rho exp heap1 heap2 val1 val2 acts1 acts2,
+    (H.empty Val, env, rho, exp) ⇓ (heap1, val1, acts1) ->
+    (H.empty Val, env, rho, exp) ⇓ (heap2, val2, acts2) ->
+    forall ctxt rgns ty static,
+      TcRho (rho, rgns) ->
+      TcEnv (ST.empty tau, rho, env, ctxt) ->
+      TcExp (ctxt, rgns, exp, ty, static) ->
+      H.Equal heap1 heap2 /\ val1 = val2 /\ acts1 = acts2.
+Proof.
+  intros.
+  eapply DynamicDeterminism_ext; eauto.
+  -  unfold H.Equal.
+     intros. 
+     apply HMapP.find_o. firstorder.
+  - assert (HH1 : forall heap stty,
+                    H.Empty heap -> ST.Empty stty -> TcHeap (heap, stty)).
+    intros; apply TcHeapEmpty; auto. 
+
+    assert (HH2 : H.Empty (elt:=Val) (H.empty Val)).
+    unfold H.Empty. simpl. 
+    unfold H.Raw.Proofs.Empty.
+    intros. intro Hneg. 
+    apply HMapP.empty_mapsto_iff in Hneg. contradiction.
+
+    assert (HH3 : ST.Empty (elt:=tau) (ST.empty tau)).
+    unfold ST.Empty. simpl. 
+    unfold ST.Raw.Proofs.Empty.
+    intros. intro Hneg. 
+    apply STMapP.empty_mapsto_iff in Hneg. contradiction.
+
+    apply HH1; auto.
+Qed.
