Makefile
@@ -107,8 +107,7 @@ VFILES:=Keys.v\
   EffectSystem.v\
   Determinism.v\
   DeterminismExt.v\
-  Correctness.v\
-  CorrectDeterminism.v
+  Correctness.v
 
 ifneq ($(filter-out archclean clean cleanall printenv,$(MAKECMDGOALS)),)
 -include $(addsuffix .d,$(VFILES))
